src/linear/interface/List3.dfy
@@ -10,24 +10,24 @@ trait ListIterator {
     requires Valid()
     requires Parent().Valid()
     ensures Index() <= |Parent().Model()|
-    ensures HasNext() <==> Index() < |Parent().Model()|
-    ensures !HasNext() <==> Index() == |Parent().Model()|
 
   function method HasNext(): bool
-    reads this
+    reads this, Parent(), Parent().Repr()
+    requires Valid()
+    requires Parent().Valid()
+    ensures HasNext() <==> Index() < |Parent().Model()|
 
   method Next() returns (x: int)
     modifies this
-    requires HasNext()
     requires Valid()
     requires Parent().Valid()
+    requires HasNext()
     requires allocated(Parent())
-    requires forall it | it in Parent().Iterators() :: allocated(it)
+    requires forall it | it in Parent().Repr() :: allocated(it)
     ensures Parent().Valid()
     ensures Valid()
     ensures old(Index()) < Index()
     ensures old(Parent()) == Parent()
-    ensures old(Index()) < |Parent().Model()|
     ensures old(Parent().Model()) == Parent().Model()
     ensures Parent().Iterators() == old(Parent().Iterators())
     ensures x == Parent().Model()[old(Index())]
@@ -106,8 +106,7 @@ trait List {
   function Iterators(): set<ListIterator>
     reads this, Repr()
     requires Valid()
-    // ensures Iterators() <= Repr();
-    ensures forall it | it in Iterators() :: it in Repr() &&  it.Parent() == this
+    ensures forall it | it in Iterators() :: it in Repr() && it.Parent() == this
 
   method Begin() returns (it: ListIterator)
     modifies this, Repr()
@@ -119,6 +118,7 @@ trait List {
     ensures Iterators() == {it} + old(Iterators())
     ensures it.Valid()
     ensures it.Index() == 0
+    ensures it.Parent() == this
     ensures forall it | it in old(Iterators()) && old(it.Valid()) ::
       it.Valid() && it.Index() == old(it.Index())
     ensures forall x | x in Repr() - old(Repr()) :: fresh(x)
@@ -143,7 +143,8 @@ trait List {
     ensures forall x | x in Repr() :: allocated(x)
 
     ensures Iterators() == old(Iterators())
-    ensures forall it | it in Iterators() && old(it.Valid()) :: it.Valid()
+    ensures forall it | it in Iterators() && old(it.Valid()) ::
+      it.Valid() // && it.Index() == old(it.Index()) + 1
 
   method PopFront() returns (x: int)
     modifies this, Repr()
@@ -162,6 +163,8 @@ trait List {
         !it.Valid()
       else
         it.Valid() && it.Index() + 1 == old(it.Index())
+    // ensures forall it | it in Iterators() && old(it.Valid()) && old(it.Index()) != 0 ::
+    //   it.Valid() && it.Index() + 1 == old(it.Index())
 
   function method Back(): int
     reads this, Repr()
@@ -181,7 +184,8 @@ trait List {
     ensures forall x | x in Repr() :: allocated(x)
 
     ensures Iterators() == old(Iterators())
-    ensures forall it | it in Iterators() && old(it.Valid()) :: it.Valid()
+    ensures forall it | it in Iterators() && old(it.Valid()) ::
+      it.Valid() // && it.Index() == old(it.Index())
 
   method PopBack() returns (x: int)
     modifies this, Repr()
@@ -204,30 +208,18 @@ trait List {
         it.Valid() && it.Index() == old(it.Index())
 }
 
-lemma Obvious(x: object)
-  ensures allocated(x)
-{}
-
-lemma Obviouss(os: set<object>)
-  ensures forall x | x in os :: allocated(x)
-{
-  forall x | x in os
-    ensures allocated(x)
-  {
-    Obvious(x);
-  }
-}
-
 method ItertatorExample1(l: List, v: array<int>)
   modifies l, l.Repr(), v
   requires {v} !! {l} + l.Repr()
   requires l.Valid()
   requires v.Length == |l.Model()|
+  requires forall x | x in l.Repr() :: allocated(x)
   ensures l.Valid()
   ensures l.Model() == old(l.Model())
   ensures v[..] == l.Model()
+  ensures forall x | x in l.Repr() - old(l.Repr()) :: fresh(x)
+  ensures forall x | x in l.Repr() :: allocated(x)
 {
-  Obviouss(l.Iterators());
   var it := l.Begin();
   var i := 0;
   while it.HasNext()
@@ -255,10 +247,12 @@ method ItertatorExample2(l: List)
   modifies l, l.Repr()
   requires l.Valid()
   requires l.Model() != []
+  requires forall x | x in l.Repr() :: allocated(x)
   ensures l.Valid()
   ensures l.Model() == old(l.Model())
+  ensures forall x | x in l.Repr() - old(l.Repr()) :: fresh(x)
+  ensures forall x | x in l.Repr() :: allocated(x)
 {
-  Obviouss(l.Iterators());
   var it1 := l.Begin();
   var x := it1.Next();
 }
@@ -267,10 +261,12 @@ method ItertatorExample3(l: List)
   modifies l, l.Repr()
   requires l.Valid()
   requires l.Model() != []
+  requires forall x | x in l.Repr() :: allocated(x)
   ensures l.Valid()
   ensures l.Model() == old(l.Model())
+  ensures forall x | x in l.Repr() - old(l.Repr()) :: fresh(x)
+  ensures forall x | x in l.Repr() :: allocated(x)
 {
-  Obviouss(l.Iterators());
   var it1 := l.Begin();
   var it2 := l.Begin();
   assert it2.Valid();
@@ -288,9 +284,11 @@ method ItertatorExample4(l: List)
   modifies l, l.Repr()
   requires l.Valid()
   requires l.Model() != []
+  requires forall x | x in l.Repr() :: allocated(x)
   ensures l.Valid()
+  ensures forall x | x in l.Repr() - old(l.Repr()) :: fresh(x)
+  ensures forall x | x in l.Repr() :: allocated(x)
 {
-  /*GHOST*/ Obviouss(l.Iterators());
   var it1 := l.Begin();
   var it2 := l.Begin();
   var x := it2.Next();
@@ -304,6 +302,7 @@ method FindMax(l: List) returns (max: ListIterator)
   modifies l, l.Repr()
   requires l.Valid()
   requires l.Model() != []
+  requires forall x | x in l.Repr() :: allocated(x)
   ensures l.Valid()
   ensures l.Model() == old(l.Model())
   ensures fresh(max)
@@ -311,8 +310,12 @@ method FindMax(l: List) returns (max: ListIterator)
   ensures max.Parent() == l
   ensures max.HasNext()
   ensures forall x | x in l.Model() :: l.Model()[max.Index()] >= x
+  ensures forall x | x in l.Repr() - old(l.Repr()) :: fresh(x)
+  ensures forall x | x in l.Repr() :: allocated(x)
+  ensures l.Iterators() >= old(l.Iterators())
+  ensures forall it | it in old(l.Iterators()) && old(it.Valid()) ::
+    it.Valid() && it.Index() == old(it.Index())
 {
-  /*GHOST*/ Obviouss(l.Iterators());
   max := l.Begin();
   var it := l.Begin();
   while it.HasNext()
@@ -332,6 +335,10 @@ method FindMax(l: List) returns (max: ListIterator)
     invariant forall k | 0 <= k < it.Index() :: l.Model()[max.Index()] >= l.Model()[k]
     invariant forall x | x in l.Repr() - old(l.Repr()) :: fresh(x)
     invariant forall x | x in l.Repr() :: allocated(x)
+    invariant forall x | x in old(l.Repr()) :: allocated(x)
+    invariant l.Iterators() >= old(l.Iterators())
+    invariant forall it | it in old(l.Iterators()) && old(it.Valid()) ::
+      it.Valid() && it.Index() == old(it.Index())
   {
     if it.Peek() > max.Peek() {
       max := it.Copy();
